Remove ndopsem and change Structure GenericValues to Module GenericValue_helper in opsem.v.

src/Vellvm/dopsem.v
@@ -27,260 +27,260 @@ Import LLVMinfra.
    semantics. *)
 
 (* DGVs implements the signature of GenericValues. *)
-Module MDGVs.
+(* Module MDGVs. *)
 
-Definition t := GenericValue.
-Definition instantiate_gvs (gv : GenericValue) (gvs : t) : Prop := gvs = gv.
-Definition inhabited (gvs : t) : Prop := True.
-Definition cundef_gvs := LLVMgv.cundef_gv.
-Definition undef_gvs gv (ty:typ) : t := gv.
-Definition cgv2gvs := LLVMgv.cgv2gv.
-Definition gv2gvs (gv:GenericValue) (ty:typ) : t := gv.
+(* Definition t := GenericValue. *)
+(* Definition instantiate_gvs (gv : GenericValue) (gvs : t) : Prop := gvs = gv. *)
+(* Definition inhabited (gvs : t) : Prop := True. *)
+(* Definition cundef_gvs := LLVMgv.cundef_gv. *)
+(* Definition undef_gvs gv (ty:typ) : t := gv. *)
+(* Definition cgv2gvs := LLVMgv.cgv2gv. *)
+(* Definition gv2gvs (gv:GenericValue) (ty:typ) : t := gv. *)
+
+(* Notation "gv @ gvs" := *)
+(*   (instantiate_gvs gv gvs) (at level 43, right associativity). *)
+(* Notation "$ gv # t $" := (gv2gvs gv t) (at level 41). *)
+(* Hint Unfold inhabited instantiate_gvs. *)
+
+(* Lemma cundef_gvs__getTypeSizeInBits : forall S los nts gv ty sz al gv', *)
+(*   wf_typ S (los,nts) ty -> *)
+(*   _getTypeSizeInBits_and_Alignment los *)
+(*     (getTypeSizeInBits_and_Alignment_for_namedts (los,nts) true) true ty = *)
+(*       Some (sz, al) -> *)
+(*   Coqlib.nat_of_Z (Coqlib.ZRdiv (Z_of_nat sz) 8) = sizeGenericValue gv -> *)
+(*   gv' @ (cundef_gvs gv ty) -> *)
+(*   Coqlib.nat_of_Z (Coqlib.ZRdiv (Z_of_nat sz) 8) = *)
+(*     sizeGenericValue gv'. *)
+(* Proof. *)
+(*   unfold instantiate_gvs. *)
+(*   intros. inv H2. *)
+(*   eapply cundef_gv__getTypeSizeInBits; eauto. *)
+(* Qed. *)
+
+(* Lemma cundef_gvs__matches_chunks : forall S los nts gv ty gv', *)
+(*   wf_typ S (los,nts) ty -> *)
+(*   gv_chunks_match_typ (los, nts) gv ty -> *)
+(*   gv' @ (cundef_gvs gv ty) -> *)
+(*   gv_chunks_match_typ (los, nts) gv' ty. *)
+(* Proof. *)
+(*   unfold instantiate_gvs. *)
+(*   intros. subst. *)
+(*   eapply cundef_gv__matches_chunks; eauto. *)
+(* Qed. *)
+
+(* Lemma cundef_gvs__inhabited : forall gv ty, inhabited (cundef_gvs gv ty). *)
+(* Proof. auto. Qed. *)
+
+(* Lemma undef_gvs__getTypeSizeInBits : forall S los nts gv t sz al gv', *)
+(*   wf_typ S (los,nts) t -> *)
+(*   _getTypeSizeInBits_and_Alignment los *)
+(*     (getTypeSizeInBits_and_Alignment_for_namedts (los,nts) true) true t = *)
+(*       Some (sz, al) -> *)
+(*   Coqlib.nat_of_Z (Coqlib.ZRdiv (Z_of_nat sz) 8) = sizeGenericValue gv -> *)
+(*   gv' @ (undef_gvs gv t) -> *)
+(*   Coqlib.nat_of_Z (Coqlib.ZRdiv (Z_of_nat sz) 8) = *)
+(*     sizeGenericValue gv'. *)
+(* Proof. *)
+(*   unfold instantiate_gvs. *)
+(*   intros. inv H2. auto. *)
+(* Qed. *)
+
+(* Lemma undef_gvs__matches_chunks : forall S los nts gv ty gv', *)
+(*   wf_typ S (los,nts) ty -> *)
+(*   gv_chunks_match_typ (los, nts) gv ty -> *)
+(*   gv' @ (undef_gvs gv ty) -> *)
+(*   gv_chunks_match_typ (los, nts) gv' ty. *)
+(* Proof. *)
+(*   unfold instantiate_gvs. *)
+(*   intros. subst. auto. *)
+(* Qed. *)
+
+(* Lemma undef_gvs__inhabited : forall gv ty, inhabited (undef_gvs gv ty). *)
+(* Proof. auto. Qed. *)
+
+(* Lemma cgv2gvs__getTypeSizeInBits : forall S los nts gv t sz al gv', *)
+(*   wf_typ S (los,nts) t -> *)
+(*   _getTypeSizeInBits_and_Alignment los *)
+(*     (getTypeSizeInBits_and_Alignment_for_namedts (los,nts) true) true t = *)
+(*       Some (sz, al) -> *)
+(*   Coqlib.nat_of_Z (Coqlib.ZRdiv (Z_of_nat sz) 8) = sizeGenericValue gv -> *)
+(*   gv' @ (cgv2gvs gv t) -> *)
+(*   Coqlib.nat_of_Z (Coqlib.ZRdiv (Z_of_nat sz) 8) = *)
+(*     sizeGenericValue gv'. *)
+(* Proof. *)
+(*   unfold instantiate_gvs. *)
+(*   intros. inv H2. *)
+(*   eapply cgv2gv__getTypeSizeInBits; eauto. *)
+(* Qed. *)
+
+(* Lemma cgv2gvs__matches_chunks : forall S los nts gv t gv', *)
+(*   wf_typ S (los,nts) t -> *)
+(*   gv_chunks_match_typ (los, nts) gv t -> *)
+(*   gv' @ (cgv2gvs gv t) -> *)
+(*   gv_chunks_match_typ (los, nts) gv' t. *)
+(* Proof. *)
+(*   unfold instantiate_gvs. *)
+(*   intros. subst. unfold cgv2gvs. *)
+(*   destruct gv; auto. *)
+(*   destruct p as [[]]; auto.  *)
+(*   destruct gv; auto. *)
+(*   eapply cundef_gvs__matches_chunks; eauto. *)
+(* Qed. *)
+
+(* Lemma cgv2gvs__inhabited : forall gv t, inhabited (cgv2gvs gv t). *)
+(* Proof. auto. Qed. *)
+
+(* Lemma gv2gvs__getTypeSizeInBits : forall S los nts gv t sz al, *)
+(*   wf_typ S (los,nts) t -> *)
+(*   _getTypeSizeInBits_and_Alignment los *)
+(*     (getTypeSizeInBits_and_Alignment_for_namedts (los,nts) true) true t = *)
+(*       Some (sz, al) -> *)
+(*   Coqlib.nat_of_Z (Coqlib.ZRdiv (Z_of_nat sz) 8) = sizeGenericValue gv -> *)
+(*   forall gv', gv' @ (gv2gvs gv t) -> *)
+(*   sizeGenericValue gv' = Coqlib.nat_of_Z (Coqlib.ZRdiv (Z_of_nat sz) 8). *)
+(* Proof. *)
+(*   unfold instantiate_gvs. *)
+(*   intros. inv H2. auto. *)
+(* Qed. *)
+
+(* Lemma gv2gvs__matches_chunks : forall S los nts gv t, *)
+(*   wf_typ S (los,nts) t -> *)
+(*   gv_chunks_match_typ (los, nts) gv t -> *)
+(*   forall gv', gv' @ (gv2gvs gv t) -> *)
+(*   gv_chunks_match_typ (los, nts) gv' t. *)
+(* Proof. *)
+(*   unfold instantiate_gvs. *)
+(*   intros. subst. auto. *)
+(* Qed. *)
+
+(* Lemma gv2gvs__inhabited : forall gv t, inhabited ($ gv # t $). *)
+(* Proof. auto. Qed. *)
+
+(* Definition lift_op1 (f: GenericValue -> option GenericValue) (gvs1:t) (ty:typ) : *)
+(*   option t := f gvs1. *)
+
+(* Definition lift_op2 (f: GenericValue -> GenericValue -> option GenericValue) *)
+(*   (gvs1 gvs2:t) (ty: typ) : option t := f gvs1 gvs2. *)
+
+(* Lemma lift_op1__inhabited : forall f gvs1 ty gvs2 *)
+(*   (H:forall x, exists z, f x = Some z), *)
+(*   inhabited gvs1 -> *)
+(*   lift_op1 f gvs1 ty = Some gvs2 -> *)
+(*   inhabited gvs2. *)
+(* Proof. auto. Qed. *)
+
+(* Lemma lift_op2__inhabited : forall f gvs1 gvs2 t gvs3 *)
+(*   (H:forall x y, exists z, f x y = Some z), *)
+(*   inhabited gvs1 -> inhabited gvs2 -> *)
+(*   lift_op2 f gvs1 gvs2 t = Some gvs3 -> *)
+(*   inhabited gvs3. *)
+(* Proof. auto. Qed. *)
+
+(* Lemma lift_op1__isnt_stuck : forall f gvs1 ty *)
+(*   (H:forall x, exists z, f x = Some z), *)
+(*   exists gvs2, lift_op1 f gvs1 ty = Some gvs2. *)
+(* Proof. unfold lift_op1. auto. Qed. *)
+
+(* Lemma lift_op2__isnt_stuck : forall f gvs1 gvs2 t *)
+(*   (H:forall x y, exists z, f x y = Some z), *)
+(*   exists gvs3, lift_op2 f gvs1 gvs2 t = Some gvs3. *)
+(* Proof. unfold lift_op2. auto. Qed. *)
+
+(* Lemma lift_op1__getTypeSizeInBits : forall S los nts f g t sz al gvs, *)
+(*   wf_typ S (los,nts) t -> *)
+(*   _getTypeSizeInBits_and_Alignment los *)
+(*     (getTypeSizeInBits_and_Alignment_for_namedts (los,nts) true) true t = *)
+(*       Some (sz, al) -> *)
+(*   (forall x y, x @ g -> f x = Some y -> *)
+(*    sizeGenericValue y = nat_of_Z (ZRdiv (Z_of_nat sz) 8)) -> *)
+(*   lift_op1 f g t = Some gvs -> *)
+(*   forall gv : GenericValue, *)
+(*   gv @ gvs -> *)
+(*   sizeGenericValue gv = nat_of_Z (ZRdiv (Z_of_nat sz) 8). *)
+(* Proof. intros. unfold lift_op1 in H2. inv H3. eauto. Qed. *)
+
+(* Lemma lift_op1__matches_chunks : forall S los nts f g t gvs, *)
+(*   wf_typ S (los,nts) t -> *)
+(*   (forall x y, instantiate_gvs x g -> f x = Some y -> *)
+(*     gv_chunks_match_typ (los, nts) y t) -> *)
+(*   lift_op1 f g t = Some gvs -> *)
+(*   forall gv : GenericValue, *)
+(*   instantiate_gvs gv gvs -> *)
+(*   gv_chunks_match_typ (los, nts) gv t. *)
+(* Proof. intros. unfold lift_op1 in H1. inv H2. eauto. Qed. *)
+
+(* Lemma lift_op2__getTypeSizeInBits : forall S los nts f g1 g2 t sz al gvs, *)
+(*   wf_typ S (los,nts) t -> *)
+(*   _getTypeSizeInBits_and_Alignment los *)
+(*     (getTypeSizeInBits_and_Alignment_for_namedts (los,nts) true) true t = *)
+(*       Some (sz, al) -> *)
+(*   (forall x y z, x @ g1 -> y @ g2 -> f x y = Some z -> *)
+(*    sizeGenericValue z = nat_of_Z (ZRdiv (Z_of_nat sz) 8)) -> *)
+(*   lift_op2 f g1 g2 t = Some gvs -> *)
+(*   forall gv : GenericValue, *)
+(*   gv @ gvs -> *)
+(*   sizeGenericValue gv = nat_of_Z (ZRdiv (Z_of_nat sz) 8). *)
+(* Proof. intros. unfold lift_op2 in H2. inv H3. eauto. Qed. *)
+
+(* Lemma lift_op2__matches_chunks : forall S los nts f g1 g2 t gvs, *)
+(*   wf_typ S (los,nts) t -> *)
+(*   (forall x y z, *)
+(*    instantiate_gvs x g1 -> instantiate_gvs y g2 -> f x y = Some z -> *)
+(*    gv_chunks_match_typ (los, nts) z t) -> *)
+(*   lift_op2 f g1 g2 t = Some gvs -> *)
+(*   forall gv : GenericValue, *)
+(*   instantiate_gvs gv gvs -> *)
+(*   gv_chunks_match_typ (los, nts) gv t. *)
+(* Proof. intros. unfold lift_op2 in H1. inv H2. eauto. Qed. *)
+
+(* Lemma inhabited_inv : forall gvs, inhabited gvs -> exists gv, gv @ gvs. *)
+(* Proof. eauto. Qed. *)
+
+(* Lemma instantiate_undef__undef_gvs : forall gv t, gv @ (undef_gvs gv t). *)
+(* Proof. auto. Qed. *)
+
+(* Lemma instantiate_gv__gv2gvs : forall gv t, gv @ ($ gv # t $). *)
+(* Proof. auto. Qed. *)
+
+(* Lemma none_undef2gvs_inv : forall gv gv' t, *)
+(*   gv @ $ gv' # t $ -> (forall mc, (Vundef, mc)::nil <> gv') -> gv = gv'. *)
+(* Proof. *)
+(*   intros. *)
+(*   destruct gv'; try solve [inv H; auto]. *)
+(* Qed. *)
+
+(* End MDGVs. *)
+
+(* Definition DGVs : GenericValues := mkGVs *)
+(* MDGVs.t *)
+(* MDGVs.instantiate_gvs *)
+(* MDGVs.inhabited *)
+(* MDGVs.cgv2gvs *)
+(* MDGVs.gv2gvs *)
+(* MDGVs.lift_op1 *)
+(* MDGVs.lift_op2 *)
+(* MDGVs.cgv2gvs__getTypeSizeInBits *)
+(* MDGVs.cgv2gvs__matches_chunks *)
+(* MDGVs.cgv2gvs__inhabited *)
+(* MDGVs.gv2gvs__getTypeSizeInBits *)
+(* MDGVs.gv2gvs__matches_chunks *)
+(* MDGVs.gv2gvs__inhabited *)
+(* MDGVs.lift_op1__inhabited *)
+(* MDGVs.lift_op2__inhabited *)
+(* MDGVs.lift_op1__isnt_stuck *)
+(* MDGVs.lift_op2__isnt_stuck *)
+(* MDGVs.lift_op1__getTypeSizeInBits *)
+(* MDGVs.lift_op2__getTypeSizeInBits *)
+(* MDGVs.lift_op1__matches_chunks *)
+(* MDGVs.lift_op2__matches_chunks *)
+(* MDGVs.inhabited_inv *)
+(* MDGVs.instantiate_gv__gv2gvs *)
+(* MDGVs.none_undef2gvs_inv. *)
 
 Notation "gv @ gvs" :=
-  (instantiate_gvs gv gvs) (at level 43, right associativity).
-Notation "$ gv # t $" := (gv2gvs gv t) (at level 41).
-Hint Unfold inhabited instantiate_gvs.
-
-Lemma cundef_gvs__getTypeSizeInBits : forall S los nts gv ty sz al gv',
-  wf_typ S (los,nts) ty ->
-  _getTypeSizeInBits_and_Alignment los
-    (getTypeSizeInBits_and_Alignment_for_namedts (los,nts) true) true ty =
-      Some (sz, al) ->
-  Coqlib.nat_of_Z (Coqlib.ZRdiv (Z_of_nat sz) 8) = sizeGenericValue gv ->
-  gv' @ (cundef_gvs gv ty) ->
-  Coqlib.nat_of_Z (Coqlib.ZRdiv (Z_of_nat sz) 8) =
-    sizeGenericValue gv'.
-Proof.
-  unfold instantiate_gvs.
-  intros. inv H2.
-  eapply cundef_gv__getTypeSizeInBits; eauto.
-Qed.
-
-Lemma cundef_gvs__matches_chunks : forall S los nts gv ty gv',
-  wf_typ S (los,nts) ty ->
-  gv_chunks_match_typ (los, nts) gv ty ->
-  gv' @ (cundef_gvs gv ty) ->
-  gv_chunks_match_typ (los, nts) gv' ty.
-Proof.
-  unfold instantiate_gvs.
-  intros. subst.
-  eapply cundef_gv__matches_chunks; eauto.
-Qed.
-
-Lemma cundef_gvs__inhabited : forall gv ty, inhabited (cundef_gvs gv ty).
-Proof. auto. Qed.
-
-Lemma undef_gvs__getTypeSizeInBits : forall S los nts gv t sz al gv',
-  wf_typ S (los,nts) t ->
-  _getTypeSizeInBits_and_Alignment los
-    (getTypeSizeInBits_and_Alignment_for_namedts (los,nts) true) true t =
-      Some (sz, al) ->
-  Coqlib.nat_of_Z (Coqlib.ZRdiv (Z_of_nat sz) 8) = sizeGenericValue gv ->
-  gv' @ (undef_gvs gv t) ->
-  Coqlib.nat_of_Z (Coqlib.ZRdiv (Z_of_nat sz) 8) =
-    sizeGenericValue gv'.
-Proof.
-  unfold instantiate_gvs.
-  intros. inv H2. auto.
-Qed.
-
-Lemma undef_gvs__matches_chunks : forall S los nts gv ty gv',
-  wf_typ S (los,nts) ty ->
-  gv_chunks_match_typ (los, nts) gv ty ->
-  gv' @ (undef_gvs gv ty) ->
-  gv_chunks_match_typ (los, nts) gv' ty.
-Proof.
-  unfold instantiate_gvs.
-  intros. subst. auto.
-Qed.
-
-Lemma undef_gvs__inhabited : forall gv ty, inhabited (undef_gvs gv ty).
-Proof. auto. Qed.
-
-Lemma cgv2gvs__getTypeSizeInBits : forall S los nts gv t sz al gv',
-  wf_typ S (los,nts) t ->
-  _getTypeSizeInBits_and_Alignment los
-    (getTypeSizeInBits_and_Alignment_for_namedts (los,nts) true) true t =
-      Some (sz, al) ->
-  Coqlib.nat_of_Z (Coqlib.ZRdiv (Z_of_nat sz) 8) = sizeGenericValue gv ->
-  gv' @ (cgv2gvs gv t) ->
-  Coqlib.nat_of_Z (Coqlib.ZRdiv (Z_of_nat sz) 8) =
-    sizeGenericValue gv'.
-Proof.
-  unfold instantiate_gvs.
-  intros. inv H2.
-  eapply cgv2gv__getTypeSizeInBits; eauto.
-Qed.
-
-Lemma cgv2gvs__matches_chunks : forall S los nts gv t gv',
-  wf_typ S (los,nts) t ->
-  gv_chunks_match_typ (los, nts) gv t ->
-  gv' @ (cgv2gvs gv t) ->
-  gv_chunks_match_typ (los, nts) gv' t.
-Proof.
-  unfold instantiate_gvs.
-  intros. subst. unfold cgv2gvs.
-  destruct gv; auto.
-  destruct p as [[]]; auto. 
-  destruct gv; auto.
-  eapply cundef_gvs__matches_chunks; eauto.
-Qed.
-
-Lemma cgv2gvs__inhabited : forall gv t, inhabited (cgv2gvs gv t).
-Proof. auto. Qed.
-
-Lemma gv2gvs__getTypeSizeInBits : forall S los nts gv t sz al,
-  wf_typ S (los,nts) t ->
-  _getTypeSizeInBits_and_Alignment los
-    (getTypeSizeInBits_and_Alignment_for_namedts (los,nts) true) true t =
-      Some (sz, al) ->
-  Coqlib.nat_of_Z (Coqlib.ZRdiv (Z_of_nat sz) 8) = sizeGenericValue gv ->
-  forall gv', gv' @ (gv2gvs gv t) ->
-  sizeGenericValue gv' = Coqlib.nat_of_Z (Coqlib.ZRdiv (Z_of_nat sz) 8).
-Proof.
-  unfold instantiate_gvs.
-  intros. inv H2. auto.
-Qed.
-
-Lemma gv2gvs__matches_chunks : forall S los nts gv t,
-  wf_typ S (los,nts) t ->
-  gv_chunks_match_typ (los, nts) gv t ->
-  forall gv', gv' @ (gv2gvs gv t) ->
-  gv_chunks_match_typ (los, nts) gv' t.
-Proof.
-  unfold instantiate_gvs.
-  intros. subst. auto.
-Qed.
-
-Lemma gv2gvs__inhabited : forall gv t, inhabited ($ gv # t $).
-Proof. auto. Qed.
-
-Definition lift_op1 (f: GenericValue -> option GenericValue) (gvs1:t) (ty:typ) :
-  option t := f gvs1.
-
-Definition lift_op2 (f: GenericValue -> GenericValue -> option GenericValue)
-  (gvs1 gvs2:t) (ty: typ) : option t := f gvs1 gvs2.
-
-Lemma lift_op1__inhabited : forall f gvs1 ty gvs2
-  (H:forall x, exists z, f x = Some z),
-  inhabited gvs1 ->
-  lift_op1 f gvs1 ty = Some gvs2 ->
-  inhabited gvs2.
-Proof. auto. Qed.
-
-Lemma lift_op2__inhabited : forall f gvs1 gvs2 t gvs3
-  (H:forall x y, exists z, f x y = Some z),
-  inhabited gvs1 -> inhabited gvs2 ->
-  lift_op2 f gvs1 gvs2 t = Some gvs3 ->
-  inhabited gvs3.
-Proof. auto. Qed.
-
-Lemma lift_op1__isnt_stuck : forall f gvs1 ty
-  (H:forall x, exists z, f x = Some z),
-  exists gvs2, lift_op1 f gvs1 ty = Some gvs2.
-Proof. unfold lift_op1. auto. Qed.
-
-Lemma lift_op2__isnt_stuck : forall f gvs1 gvs2 t
-  (H:forall x y, exists z, f x y = Some z),
-  exists gvs3, lift_op2 f gvs1 gvs2 t = Some gvs3.
-Proof. unfold lift_op2. auto. Qed.
-
-Lemma lift_op1__getTypeSizeInBits : forall S los nts f g t sz al gvs,
-  wf_typ S (los,nts) t ->
-  _getTypeSizeInBits_and_Alignment los
-    (getTypeSizeInBits_and_Alignment_for_namedts (los,nts) true) true t =
-      Some (sz, al) ->
-  (forall x y, x @ g -> f x = Some y ->
-   sizeGenericValue y = nat_of_Z (ZRdiv (Z_of_nat sz) 8)) ->
-  lift_op1 f g t = Some gvs ->
-  forall gv : GenericValue,
-  gv @ gvs ->
-  sizeGenericValue gv = nat_of_Z (ZRdiv (Z_of_nat sz) 8).
-Proof. intros. unfold lift_op1 in H2. inv H3. eauto. Qed.
-
-Lemma lift_op1__matches_chunks : forall S los nts f g t gvs,
-  wf_typ S (los,nts) t ->
-  (forall x y, instantiate_gvs x g -> f x = Some y ->
-    gv_chunks_match_typ (los, nts) y t) ->
-  lift_op1 f g t = Some gvs ->
-  forall gv : GenericValue,
-  instantiate_gvs gv gvs ->
-  gv_chunks_match_typ (los, nts) gv t.
-Proof. intros. unfold lift_op1 in H1. inv H2. eauto. Qed.
-
-Lemma lift_op2__getTypeSizeInBits : forall S los nts f g1 g2 t sz al gvs,
-  wf_typ S (los,nts) t ->
-  _getTypeSizeInBits_and_Alignment los
-    (getTypeSizeInBits_and_Alignment_for_namedts (los,nts) true) true t =
-      Some (sz, al) ->
-  (forall x y z, x @ g1 -> y @ g2 -> f x y = Some z ->
-   sizeGenericValue z = nat_of_Z (ZRdiv (Z_of_nat sz) 8)) ->
-  lift_op2 f g1 g2 t = Some gvs ->
-  forall gv : GenericValue,
-  gv @ gvs ->
-  sizeGenericValue gv = nat_of_Z (ZRdiv (Z_of_nat sz) 8).
-Proof. intros. unfold lift_op2 in H2. inv H3. eauto. Qed.
-
-Lemma lift_op2__matches_chunks : forall S los nts f g1 g2 t gvs,
-  wf_typ S (los,nts) t ->
-  (forall x y z,
-   instantiate_gvs x g1 -> instantiate_gvs y g2 -> f x y = Some z ->
-   gv_chunks_match_typ (los, nts) z t) ->
-  lift_op2 f g1 g2 t = Some gvs ->
-  forall gv : GenericValue,
-  instantiate_gvs gv gvs ->
-  gv_chunks_match_typ (los, nts) gv t.
-Proof. intros. unfold lift_op2 in H1. inv H2. eauto. Qed.
-
-Lemma inhabited_inv : forall gvs, inhabited gvs -> exists gv, gv @ gvs.
-Proof. eauto. Qed.
-
-Lemma instantiate_undef__undef_gvs : forall gv t, gv @ (undef_gvs gv t).
-Proof. auto. Qed.
-
-Lemma instantiate_gv__gv2gvs : forall gv t, gv @ ($ gv # t $).
-Proof. auto. Qed.
-
-Lemma none_undef2gvs_inv : forall gv gv' t,
-  gv @ $ gv' # t $ -> (forall mc, (Vundef, mc)::nil <> gv') -> gv = gv'.
-Proof.
-  intros.
-  destruct gv'; try solve [inv H; auto].
-Qed.
-
-End MDGVs.
-
-Definition DGVs : GenericValues := mkGVs
-MDGVs.t
-MDGVs.instantiate_gvs
-MDGVs.inhabited
-MDGVs.cgv2gvs
-MDGVs.gv2gvs
-MDGVs.lift_op1
-MDGVs.lift_op2
-MDGVs.cgv2gvs__getTypeSizeInBits
-MDGVs.cgv2gvs__matches_chunks
-MDGVs.cgv2gvs__inhabited
-MDGVs.gv2gvs__getTypeSizeInBits
-MDGVs.gv2gvs__matches_chunks
-MDGVs.gv2gvs__inhabited
-MDGVs.lift_op1__inhabited
-MDGVs.lift_op2__inhabited
-MDGVs.lift_op1__isnt_stuck
-MDGVs.lift_op2__isnt_stuck
-MDGVs.lift_op1__getTypeSizeInBits
-MDGVs.lift_op2__getTypeSizeInBits
-MDGVs.lift_op1__matches_chunks
-MDGVs.lift_op2__matches_chunks
-MDGVs.inhabited_inv
-MDGVs.instantiate_gv__gv2gvs
-MDGVs.none_undef2gvs_inv.
-
-Notation "gv @ gvs" :=
-  (DGVs.(instantiate_gvs) gv gvs) (at level 43, right associativity).
-Notation "$ gv # t $" := (DGVs.(gv2gvs) gv t) (at level 41).
-Notation "vidxs @@ vidxss" := (@Opsem.in_list_gvs DGVs vidxs vidxss)
+  (GenericValue_helper.instantiate_gvs gv gvs) (at level 43, right associativity).
+Notation "$ gv # t $" := (GenericValue_helper.gv2gvs gv t) (at level 41).
+Notation "vidxs @@ vidxss" := (Opsem.in_list_gvs vidxs vidxss)
   (at level 43, right associativity).
 
 (* Properties of deterministic operational semantics. *)
@@ -297,15 +297,13 @@ Qed.
 
 Ltac dgvs_instantiate_inv :=
   match goal with
-  | [ H : DGVs.(instantiate_gvs) _ _ |- _ ] => inv H
+  | [ H : GenericValue_helper.instantiate_gvs _ _ |- _ ] => inv H
   | [ H : _ @@ _ |- _ ] => apply dos_in_list_gvs_inv in H; subst
   end.
 
 Lemma dos_instantiate_gvs_intro : forall gv, gv @ gv.
 Proof.
-Local Transparent instantiate_gvs.
-  unfold instantiate_gvs. simpl. auto.
-Global Opaque instantiate_gvs.
+  unfold GenericValue_helper.instantiate_gvs. simpl. auto.
 Qed.
 
 Hint Resolve dos_instantiate_gvs_intro.
@@ -318,12 +316,12 @@ Qed.
 Hint Resolve dos_in_list_gvs_intro.
 
 (*************************************)
-Definition DGVMap := @Opsem.GVsMap DGVs.
+Definition DGVMap := Opsem.GVsMap.
 
 (*************************************)
 (* Aux invariants of wf ECs *)
 
-Definition wfEC_inv s m (EC: @Opsem.ExecutionContext DGVs) : Prop :=
+Definition wfEC_inv s m (EC: Opsem.ExecutionContext) : Prop :=
 uniqFdef (Opsem.CurFunction EC) /\ 
 blockInFdefB (Opsem.CurBB EC) (Opsem.CurFunction EC) = true /\
 match Opsem.CurCmds EC with
@@ -336,7 +334,7 @@ exists l0, exists ps0, exists cs0,
   Opsem.CurBB EC = (l0, stmts_intro ps0 (cs0 ++ Opsem.CurCmds EC)
     (Opsem.Terminator EC)).
 
-Definition wfECs_inv s m (ECs: list (@Opsem.ExecutionContext DGVs)) : Prop :=
+Definition wfECs_inv s m (ECs: list Opsem.ExecutionContext) : Prop :=
 List.Forall (wfEC_inv s m) ECs.
 
 Lemma wf_EC__wfEC_inv: forall S los nts Ps EC
@@ -389,14 +387,14 @@ Proof.
   simpl; split; auto.
 Qed.
 
-Definition uniqEC (EC: @Opsem.ExecutionContext DGVs) : Prop :=
+Definition uniqEC (EC: Opsem.ExecutionContext) : Prop :=
 uniqFdef (Opsem.CurFunction EC) /\ 
 blockInFdefB (Opsem.CurBB EC) (Opsem.CurFunction EC) = true /\
 exists l0, exists ps0, exists cs0,
   Opsem.CurBB EC = (l0, stmts_intro ps0 (cs0 ++ Opsem.CurCmds EC)
     (Opsem.Terminator EC)).
 
-Definition uniqECs (ECs: list (@Opsem.ExecutionContext DGVs)) : Prop :=
+Definition uniqECs (ECs: list Opsem.ExecutionContext) : Prop :=
 List.Forall uniqEC ECs.
 
 Lemma wfEC_inv__uniqEC: forall s m EC (Hwf: wfEC_inv s m EC), uniqEC EC.
@@ -441,16 +439,15 @@ end.
 (*************************************)
 (* More dynamic properties *)
 
-Lemma GEP_inv: forall TD t (mp1 : GVsT DGVs) inbounds0 vidxs mp2 t'
+Lemma GEP_inv: forall TD t (mp1 : GenericValue) inbounds0 vidxs mp2 t'
   (H1 : Opsem.GEP TD t mp1 vidxs inbounds0 t' = ret mp2),
   gundef TD (typ_pointer t') = ret mp2 \/
   exists blk, exists ofs1, exists ofs2 : int32, exists m1, exists m2,
     mp1 = (Vptr blk ofs1, m1) :: nil /\ mp2 = (Vptr blk ofs2, m2) :: nil.
 Proof.
-Local Transparent lift_op1.
   intros.
-  unfold Opsem.GEP in H1. unfold lift_op1 in H1. simpl in H1.
-  unfold MDGVs.lift_op1 in H1.
+  unfold Opsem.GEP in H1. unfold GenericValue_helper.lift_op1 in H1. simpl in H1.
+  unfold GenericValue_helper.lift_op1 in H1.
   unfold gep in H1. unfold GEP in H1.
   remember (GV2ptr TD (getPointerSize TD) mp1) as R1.
   destruct R1; auto.
@@ -471,7 +468,6 @@ Local Transparent lift_op1.
   exists (Int.add 31 i1 (Int.repr 31 z0)). exists m.
   exists (AST.Mint (Size.mul Size.Eight (getPointerSize TD) - 1)).
   eauto.
-Opaque lift_op1.
 Qed.
 
 Lemma wf__getTypeStoreSize_eq_sizeGenericValue: forall (gl2 : GVMap)
@@ -479,7 +475,7 @@ Lemma wf__getTypeStoreSize_eq_sizeGenericValue: forall (gl2 : GVMap)
   (Ps : list product) (v1 : value) (gv1 : GenericValue)
   (Hwfg : LLVMgv.wf_global (los, nts) S gl2) (n : nat) t
   (HeqR : ret n = getTypeStoreSize (los, nts) t) F
-  (H24 : @Opsem.getOperandValue DGVs (los, nts) v1 lc2 gl2 = ret gv1)
+  (H24 : Opsem.getOperandValue (los, nts) v1 lc2 gl2 = ret gv1)
   (Hwflc1 : OpsemPP.wf_lc (los, nts) F lc2)
   (Hwfv : wf_value S (module_intro los nts Ps) F v1 t),
   n = sizeGenericValue gv1.
