src/Vellvm/opsem_wf.v
@@ -32,17 +32,15 @@ Require Import util.
 
 Module OpsemPP. Section OpsemPP.
 
-Context `{GVsSig : GenericValues}.
-
 Export Opsem.
 Export OpsemProps.
 Import AtomSet.
 
 (* Notations *)
-Notation GVs := GVsSig.(GVsT).
+
 Notation "gv @ gvs" :=
-  (GVsSig.(instantiate_gvs) gv gvs) (at level 43, right associativity).
-Notation "$ gv # t $" := (GVsSig.(gv2gvs) gv t) (at level 41).
+  (GenericValue_helper.instantiate_gvs gv gvs) (at level 43, right associativity).
+Notation "$ gv # t $" := (GenericValue_helper.gv2gvs gv t) (at level 41).
 Notation "vidxs @@ vidxss" := (in_list_gvs vidxs vidxss)
   (at level 43, right associativity).
 
@@ -50,12 +48,12 @@ Notation "vidxs @@ vidxss" := (in_list_gvs vidxs vidxss)
    1) all values in the set are of size t;
    2) the set is not empty;
    3) all values match type t. *)
-Inductive wf_GVs : TargetData -> GVs -> typ -> Prop :=
+Inductive wf_GVs : TargetData -> GenericValue -> typ -> Prop :=
 | wf_GVs_intro : forall TD gvs t sz,
     getTypeSizeInBits TD t = Some sz ->
     (forall gv, gv @ gvs ->
       sizeGenericValue gv = Coqlib.nat_of_Z (Coqlib.ZRdiv (Z_of_nat sz) 8)) ->
-    GVsSig.(inhabited) gvs ->
+    GenericValue_helper.inhabited gvs ->
     (forall gv, gv @ gvs -> gv_chunks_match_typ TD gv t) ->
     wf_GVs TD gvs t.
 
@@ -114,7 +112,7 @@ b = (l1, stmts_intro ps (cs'++cs) tmn).
 
 (* If the current ec's current block ends with return, the next ec's
    current command must be a call. *)
-Definition wf_call (ec:@ExecutionContext GVsSig) (ecs:@ECStack GVsSig) : Prop :=
+Definition wf_call (ec:@ExecutionContext) (ecs:@ECStack) : Prop :=
 let '(mkEC f _ _ _ _ _) := ec in
 forall b, blockInFdefB b f ->
 let '(_, stmts_intro _ _ tmn) := b in
@@ -157,28 +155,22 @@ moduleInSystemB (module_intro los nts ps) s = true.
 
 (* Properties of inhabited *)
 Lemma const2GV__inhabited : forall TD gl c gvs,
-  const2GV TD gl c = Some gvs -> GVsSig.(inhabited) gvs.
+  const2GV TD gl c = Some gvs -> GenericValue_helper.inhabited gvs.
 Proof.
   intros TD gl c gvs H.
   unfold const2GV in H.
   destruct (_const2GV TD gl c) as [[gv ?]|]; inv H.
-    eauto using GVsSig.(cgv2gvs__inhabited).
+    eauto using GenericValue_helper.cgv2gvs__inhabited.
 Qed.
 
 Lemma getOperandValue__inhabited : forall los nts s ps f v t lc gl gvs,
   wf_lc (los, nts) f lc ->
   wf_value s (module_intro los nts ps) f v t ->
   getOperandValue (los, nts) v lc gl = Some gvs ->
-  GVsSig.(inhabited) gvs.
+  GenericValue_helper.inhabited gvs.
 Proof.
   intros los nts s ps f v t lc gl gvs Hwflc Hwfv Hget.
   inv Hwfv; simpl in Hget; eauto using const2GV__inhabited.
-    unfold wf_lc in Hwflc.
-    match goal with
-    | H7: lookupTypViaIDFromFdef _ _ = _ |- _ =>
-      eapply Hwflc in H7; eauto;
-      inv H7; auto
-    end.
 Qed.
 
 Lemma values2GVs__inhabited : forall S los nts f lc (Hwflc: wf_lc (los,nts) f lc)
@@ -203,9 +195,6 @@ Proof.
     rewrite wf_value_list_cons_iff in Hwfvs. destruct Hwfvs.
     destruct (@IHidxs l0) as [vidxs0 J]; auto.
     eapply getOperandValue__inhabited in HeqR; eauto.
-    apply GVsSig.(inhabited_inv) in HeqR.
-    destruct HeqR as [gv HeqR].
-    exists (gv::vidxs0). simpl. simpl; auto.
 Qed.
 
 (* Properties of type size *)
@@ -230,7 +219,7 @@ Proof.
   exists sz.
   rewrite J1.
   split; auto.
-    eapply GVsSig.(cgv2gvs__getTypeSizeInBits); eauto using wf_const__wf_typ.
+    eapply GenericValue_helper.cgv2gvs__getTypeSizeInBits; eauto using wf_const__wf_typ.
 Qed.
 
 (* Properties of matching chunks *)
@@ -249,7 +238,7 @@ Proof.
   destruct TD.
   eapply const2GV__matches_chunks_aux in HeqR; eauto.
   destruct HeqR as [J1 J2]; subst.
-  eapply GVsSig.(cgv2gvs__matches_chunks); eauto using wf_const__wf_typ.
+  eapply GenericValue_helper.cgv2gvs__matches_chunks; eauto using wf_const__wf_typ.
 Qed.
 
 (* Properties of wf_gvs *)
@@ -269,7 +258,7 @@ Proof.
     eapply wf_typ__getTypeSizeInBits_and_Alignment in H7; eauto.
     destruct H7 as [sz [al [J1 J2]]].
     eapply wf_GVs_intro with (sz:=sz);
-      eauto using GVsSig.(cgv2gvs__getTypeSizeInBits).
+      eauto using GenericValue_helper.cgv2gvs__getTypeSizeInBits.
       unfold getTypeSizeInBits, getTypeSizeInBits_and_Alignment,
              getTypeSizeInBits_and_Alignment_for_namedts in *.
       rewrite J1. auto.
@@ -477,7 +466,7 @@ Proof.
       rewrite <- lookupAL_updateAddAL_neq; eauto.
 Qed.
 
-Fixpoint wf_params TD (gvs:list GVs) (lp:params) : Prop :=
+Fixpoint wf_params TD (gvs:list GenericValue) (lp:params) : Prop :=
 match (gvs, lp) with
 | (nil, nil) => True
 | (gv::gvs', ((t, _), _)::lp') => wf_GVs TD gv t /\ wf_params TD gvs' lp'
@@ -523,7 +512,7 @@ Proof.
 Qed.
 
 Lemma wf_params_spec : forall TD gvs lp,
-  wf_params TD gvs lp -> forall gv, In gv gvs -> GVsSig.(inhabited) gv.
+  wf_params TD gvs lp -> forall gv, In gv gvs -> GenericValue_helper.inhabited gv.
 Proof.
   induction gvs; simpl; intros.
     inv H0.
@@ -531,7 +520,6 @@ Proof.
     destruct lp as [|[[]]]; tinv H.
     destruct H as [J1 J2].
     destruct H0 as [H0 | H0]; subst; eauto.
-      inv J1; auto.
 Qed.
 
 (* Properties of wf_defs *)
@@ -855,9 +843,8 @@ Proof.
     unfold getTypeSizeInBits, getTypeSizeInBits_and_Alignment,
            getTypeSizeInBits_and_Alignment_for_namedts.
     rewrite J1. auto.
-    eapply GVsSig.(gv2gvs__getTypeSizeInBits); eauto.
-    eapply GVsSig.(gv2gvs__inhabited); eauto.
-    eapply GVsSig.(gv2gvs__matches_chunks); eauto.
+    eapply GenericValue_helper.gv2gvs__getTypeSizeInBits; eauto.
+    eapply GenericValue_helper.gv2gvs__matches_chunks; eauto.
       eapply gundef__matches_chunks in J; eauto.
 Qed.
 
@@ -877,17 +864,15 @@ Proof.
            (_getTypeSizeInBits_and_Alignment_for_namedts los nts true)
            true t) as R.
     destruct R as [[]|]; inv J1.
-    eapply GVsSig.(gv2gvs__getTypeSizeInBits); eauto.
+    eapply GenericValue_helper.gv2gvs__getTypeSizeInBits; eauto.
 
-    eapply GVsSig.(gv2gvs__inhabited); eauto.
-
-    eapply GVsSig.(gv2gvs__matches_chunks); eauto.
+    eapply GenericValue_helper.gv2gvs__matches_chunks; eauto.
       eapply fit_gv__matches_chunks in J; eauto.
 Qed.
 
 Lemma lift_fit_gv__wf_gvs : forall los nts g s t t0 gv
   (Hwft : wf_typ s (los, nts) t) (Hwfg : wf_GVs (los, nts) g t0)
-  (HeqR : GVsSig.(lift_op1) (fit_gv (los, nts) t) g t = Some gv),
+  (HeqR : GenericValue_helper.lift_op1 (fit_gv (los, nts) t) g t = Some gv),
   wf_GVs (los, nts) gv t.
 Proof.
   intros.
@@ -899,7 +884,7 @@ Proof.
            getTypeSizeInBits_and_Alignment_for_namedts in *.
     rewrite J1. auto.
 
-    eapply GVsSig.(lift_op1__getTypeSizeInBits); eauto.
+    eapply GenericValue_helper.lift_op1__getTypeSizeInBits; eauto.
     intros. symmetry in H0.
     eapply fit_gv__getTypeSizeInBits in H0; eauto.
     destruct H0 as [sz0 [H1 H2]].
@@ -907,11 +892,7 @@ Proof.
     rewrite J1 in H1. inv H1. auto.
 
     inv Hwfg.
-    eapply GVsSig.(lift_op1__inhabited) in HeqR; eauto.
-    intro x. eapply fit_gv__total; eauto.
-
-    inv Hwfg.
-    eapply GVsSig.(lift_op1__matches_chunks); eauto.
+    eapply GenericValue_helper.lift_op1__matches_chunks; eauto.
     intros.
     eapply fit_gv__matches_chunks; eauto.
 Qed.
@@ -957,7 +938,7 @@ Proof.
 
       remember (_initializeFrameValues (los,nts) la2 gvs2 lc1) as R1.
       destruct R1 as [lc'|]; tinv Hin.
-      remember (GVsSig.(lift_op1) (fit_gv (los, nts) t) g t) as R2.
+      remember (GenericValue_helper.lift_op1 (fit_gv (los, nts) t) g t) as R2.
       destruct R2 as [gv|]; inv Hin.
       destruct lp2 as [|[[]]]; tinv Hpar.
       destruct Hpar as [Hwfg Hpar].
@@ -1047,7 +1028,7 @@ Proof.
   destruct R; tinv H1.
   destruct_cmd c; inv H1; auto.
   destruct n; inv H7; auto.
-  remember (GVsSig.(lift_op1) (fit_gv (los, nts) t1) g t1) as R.
+  remember (GenericValue_helper.lift_op1 (fit_gv (los, nts) t1) g t1) as R.
   destruct R; inv H6.
     eapply wf_lc_updateAddAL with (t:=t1); eauto.
       eapply uniqF__lookupTypViaIDFromFdef; eauto.
@@ -1079,16 +1060,12 @@ Proof.
     unfold getTypeSizeInBits. simpl. eauto.
 
     intros gv Hin.
-    eapply GVsSig.(lift_op2__getTypeSizeInBits) with (los:=los)(nts:=nts); eauto.
+    eapply GenericValue_helper.lift_op2__getTypeSizeInBits with (los:=los)(nts:=nts); eauto.
       simpl. eauto.
       intros. erewrite mbop_typsize; eauto.
 
-    eapply GVsSig.(lift_op2__inhabited) in H0;
-      eauto using getOperandValue__inhabited.
-    eapply mbop_is_total; eauto.
-
     intros gv Hin.
-    eapply GVsSig.(lift_op2__matches_chunks) with (los:=los)(nts:=nts); eauto.
+    eapply GenericValue_helper.lift_op2__matches_chunks with (los:=los)(nts:=nts); eauto.
       simpl. eauto.
       intros. eapply mbop_matches_chunks; eauto.
 Qed.
@@ -1114,7 +1091,7 @@ Proof.
     unfold getTypeSizeInBits. rewrite H1. auto.
 
     intros gv Hin.
-    eapply GVsSig.(lift_op2__getTypeSizeInBits) with (los:=los)(nts:=nts); eauto.
+    eapply GenericValue_helper.lift_op2__getTypeSizeInBits with (los:=los)(nts:=nts); eauto.
       simpl. eauto.
 
       intros x y z ? ? J3.
@@ -1124,12 +1101,8 @@ Proof.
       unfold getTypeSizeInBits_and_Alignment_for_namedts in *.
       rewrite H1 in J5. inv J5. auto.
 
-    eapply GVsSig.(lift_op2__inhabited) in H0;
-      eauto using getOperandValue__inhabited.
-    eapply mfbop_is_total; eauto.
-
     intros gv Hin.
-    eapply GVsSig.(lift_op2__matches_chunks) with (los:=los)(nts:=nts); eauto.
+    eapply GenericValue_helper.lift_op2__matches_chunks with (los:=los)(nts:=nts); eauto.
       intros. eapply mfbop_matches_chunks; eauto.
 Qed.
 
@@ -1150,18 +1123,13 @@ Proof.
   destruct R2; inv Hiop.
   eapply wf_GVs_intro with (sz:=Size.to_nat Size.One); eauto.
     intros gv Hin.
-    eapply GVsSig.(lift_op2__getTypeSizeInBits) with (los:=los)(nts:=nts)(S:=S);
+    eapply GenericValue_helper.lift_op2__getTypeSizeInBits with (los:=los)(nts:=nts)(S:=S);
       eauto.
       simpl. eauto.
       intros. unfold Size.to_nat. erewrite micmp_typsize; eauto.
 
-    apply GVsSig.(lift_op2__inhabited) in H0;
-      eauto using getOperandValue__inhabited.
-    apply wf_value__wf_typ in Hwfv1. destruct Hwfv1.
-    eapply micmp_is_total; eauto.
-
     intros gv Hin.
-    eapply GVsSig.(lift_op2__matches_chunks) with (los:=los)(nts:=nts); eauto.
+    eapply GenericValue_helper.lift_op2__matches_chunks with (los:=los)(nts:=nts); eauto.
       intros. eapply micmp_matches_chunks; eauto.
 Qed.
 
@@ -1182,23 +1150,18 @@ Proof.
   destruct R2; inv Hiop.
   eapply wf_GVs_intro with (sz:=Size.to_nat Size.One); eauto.
     intros gv Hin.
-    eapply GVsSig.(lift_op2__getTypeSizeInBits) with (los:=los)(nts:=nts)(S:=S);
+    eapply GenericValue_helper.lift_op2__getTypeSizeInBits with (los:=los)(nts:=nts)(S:=S);
       eauto.
       simpl. eauto.
       intros. unfold Size.to_nat. erewrite mfcmp_typsize; eauto.
 
-    apply GVsSig.(lift_op2__inhabited) in H0;
-      eauto using getOperandValue__inhabited.
-    apply wf_value__wf_typ in Hwfv1. destruct Hwfv1.
-    eapply mfcmp_is_total; eauto.
-
     intros gv Hin.
-    eapply GVsSig.(lift_op2__matches_chunks) with (los:=los)(nts:=nts); eauto.
+    eapply GenericValue_helper.lift_op2__matches_chunks with (los:=los)(nts:=nts); eauto.
       intros. eapply mfcmp_matches_chunks; eauto.
 Qed.
 
 Lemma GEP__wf_gvs : forall S TD t mp vidxs inbounds0 mp' vidxs0 t' gl lc idxs,
-  @values2GVs GVsSig TD idxs lc gl = Some vidxs ->
+  @values2GVs TD idxs lc gl = Some vidxs ->
   wf_GVs TD mp (typ_pointer t) -> vidxs0 @@ vidxs ->
   wf_typ S TD (typ_pointer t') ->
   getGEPTyp idxs t = ret (typ_pointer t') ->
@@ -1215,7 +1178,7 @@ Proof.
   destruct TD as [los nts].
   apply wf_GVs_intro with (sz:=32%nat); auto.
     intros gv Hin'.
-    eapply GVsSig.(lift_op1__getTypeSizeInBits) with (los:=los)(nts:=nts)
+    eapply GenericValue_helper.lift_op1__getTypeSizeInBits with (los:=los)(nts:=nts)
       (f:=gep (los, nts) t vidxs0 inbounds0 t') (g:=mp)
       (S:=S)(t:=typ_pointer t'); eauto.
       simpl. auto.
@@ -1230,12 +1193,8 @@ Proof.
       destruct (mgep (los, nts) t v0 l0); eauto.
         inv J3. unfold ptr2GV, val2GV. simpl. auto.
 
-    inv Hwfgv.
-    eapply GVsSig.(lift_op1__inhabited) in H0; eauto.
-    unfold gep. intro. eapply GEP_is_total; eauto.
-
     intros gv Hin'.
-    eapply GVsSig.(lift_op1__matches_chunks) with (los:=los)(nts:=nts)
+    eapply GenericValue_helper.lift_op1__matches_chunks with (los:=los)(nts:=nts)
       (f:=gep (los, nts) t vidxs0 inbounds0 t')(S:=S)
       (t:=typ_pointer t'); eauto.
       unfold gep. intros. eapply GEP_matches_chunks; eauto.
@@ -1259,7 +1218,7 @@ Proof.
     eapply getOperandValue__wf_gvs in HeqR1; eauto.
     eapply wf_GVs_intro with (sz:=sz5); eauto.
       intros gv Hin.
-      eapply GVsSig.(lift_op1__getTypeSizeInBits)with (los:=los)(nts:=nts);eauto.
+      eapply GenericValue_helper.lift_op1__getTypeSizeInBits with (los:=los)(nts:=nts);eauto.
         simpl. eauto.
 
         intros x y ? J2.
@@ -1268,18 +1227,14 @@ Proof.
         destruct J2 as [sz1 [al1 [J4 J5]]].
         simpl in J4. inv J4. auto.
 
-      inv HeqR1.
-      eapply GVsSig.(lift_op1__inhabited) in H0; eauto.
-        intro. eapply gundef__total; eauto.
-
       intros.
-      eapply GVsSig.(lift_op1__matches_chunks)with (los:=los)(nts:=nts); eauto.
+      eapply GenericValue_helper.lift_op1__matches_chunks with (los:=los)(nts:=nts); eauto.
         intros. eapply gundef__matches_chunks; eauto.
 
     eapply getOperandValue__wf_gvs in HeqR1; eauto.
     eapply wf_GVs_intro with (sz:=32%nat); eauto.
       intros gv Hin.
-      eapply GVsSig.(lift_op1__getTypeSizeInBits)with (los:=los)(nts:=nts);eauto.
+      eapply GenericValue_helper.lift_op1__getTypeSizeInBits with (los:=los)(nts:=nts);eauto.
         simpl. eauto.
 
         intros x y ? J2.
@@ -1288,30 +1243,22 @@ Proof.
         destruct J2 as [sz1 [al1 [J4 J5]]].
         simpl in J4. inv J4. auto.
 
-      inv HeqR1.
-      eapply GVsSig.(lift_op1__inhabited) in H0; eauto.
-        intro. eapply gundef__total; eauto.
-
       intros.
-      eapply GVsSig.(lift_op1__matches_chunks)with (los:=los)(nts:=nts); eauto.
+      eapply GenericValue_helper.lift_op1__matches_chunks with (los:=los)(nts:=nts); eauto.
         intros. eapply gundef__matches_chunks; eauto.
 
     eapply getOperandValue__wf_gvs in HeqR1; eauto.
     eapply wf_GVs_intro with (sz:=32%nat); eauto.
       intros gv Hin.
-      eapply GVsSig.(lift_op1__getTypeSizeInBits)with(los:=los)(nts:=nts) in Hin;
+      eapply GenericValue_helper.lift_op1__getTypeSizeInBits with(los:=los)(nts:=nts) in Hin;
         eauto.
         simpl. eauto.
         intros x y Hin' Heq. inv Heq.
         inv HeqR1.
         unfold getTypeSizeInBits in H. inv H. simpl in *. eauto.
 
-      inv HeqR1.
-      eapply GVsSig.(lift_op1__inhabited) in H0; eauto.
-        unfold mcast, mbitcast. eauto.
-
       intros.
-      eapply GVsSig.(lift_op1__matches_chunks)with (los:=los)(nts:=nts); eauto.
+      eapply GenericValue_helper.lift_op1__matches_chunks with (los:=los)(nts:=nts); eauto.
         unfold mcast, mbitcast. intros.
         inv HeqR1.
         apply H6 in H1. uniq_result.
@@ -1343,7 +1290,7 @@ Proof.
     rewrite J3. auto.
 
     intros gv Hin.
-    eapply GVsSig.(lift_op1__getTypeSizeInBits) with (los:=los)(nts:=nts); eauto.
+    eapply GenericValue_helper.lift_op1__getTypeSizeInBits with (los:=los)(nts:=nts); eauto.
       intros x y Hin' J2'.
       eapply mtrunc_typsize in J2'; eauto.
       destruct J2' as [sz' [al' [J2' J4']]].
@@ -1351,15 +1298,12 @@ Proof.
       unfold layouts, namedts in *.
       rewrite J3 in J2'. inv J2'. auto.
 
-    eapply GVsSig.(lift_op1__inhabited) in H0; eauto.
-      eapply mtrunc_is_total; eauto.
-
       symmetry in HeqR1.
       eapply getOperandValue__wf_gvs in HeqR1; eauto using wf_trunc__wf_value.
       inv HeqR1; auto.
 
     intros gv Hin.
-    eapply GVsSig.(lift_op1__matches_chunks) with (los:=los)(nts:=nts); eauto.
+    eapply GenericValue_helper.lift_op1__matches_chunks with (los:=los)(nts:=nts); eauto.
       intros x y Hin' J2'.
       eapply mtrunc_matches_chunks in J2'; eauto.
 Qed.
@@ -1387,7 +1331,7 @@ Proof.
     rewrite J4. auto.
 
     intros gv Hin.
-    eapply GVsSig.(lift_op1__getTypeSizeInBits) with (los:=los)(nts:=nts); eauto.
+    eapply GenericValue_helper.lift_op1__getTypeSizeInBits with (los:=los)(nts:=nts); eauto.
       intros x y Hin' J2'.
       eapply mext_typsize in J2'; eauto.
       destruct J2' as [sz' [al' [J2' J4']]].
@@ -1395,15 +1339,8 @@ Proof.
       unfold layouts, namedts in *.
       rewrite J4 in J2'. inv J2'. auto.
 
-    eapply GVsSig.(lift_op1__inhabited) in H0; eauto.
-      eapply mext_is_total; eauto.
-
-      symmetry in HeqR1.
-      eapply getOperandValue__wf_gvs in HeqR1; eauto using wf_ext__wf_value.
-      inv HeqR1; auto.
-
     intros gv Hin.
-    eapply GVsSig.(lift_op1__matches_chunks) with (los:=los)(nts:=nts); eauto.
+    eapply GenericValue_helper.lift_op1__matches_chunks with (los:=los)(nts:=nts); eauto.
       intros x y Hin' J2'.
       eapply mext_matches_chunks in J2'; eauto.
 Qed.
@@ -1445,7 +1382,7 @@ Proof.
     inv_mbind.
     uniq_result. symmetry_ctx. uniq_result.
     intros gv0 Hin.
-    eapply GVsSig.(lift_op2__getTypeSizeInBits)with (los:=los)(nts:=nts)(t:=t1);
+    eapply GenericValue_helper.lift_op2__getTypeSizeInBits with (los:=los)(nts:=nts)(t:=t1);
       eauto.
       intros x y z0 J4 J5 J6.
       apply H1 in J4. apply H5 in J5.
@@ -1463,14 +1400,8 @@ Proof.
           symmetry_ctx; uniq_result; auto
         end.
 
-    match goal with
-    | H6: lift_op2 _ _ _ _ _ = _ |- _ =>
-      eapply GVsSig.(lift_op2__inhabited) in H6; try solve [
-        eauto | eapply mset'_is_total; eauto]
-    end.
-
     intros gv0 Hin.
-    eapply GVsSig.(lift_op2__matches_chunks)with (los:=los)(nts:=nts)(t:=t1);
+    eapply GenericValue_helper.lift_op2__matches_chunks with (los:=los)(nts:=nts)(t:=t1);
       eauto.
       intros. apply H3 in H8. apply H7 in H9.  eapply mset'_matches_chunks; eauto.
 Qed.
@@ -1501,7 +1432,7 @@ Proof.
     rewrite J2. auto.
 
     intros gv0 Hin.
-    eapply GVsSig.(lift_op1__getTypeSizeInBits) with (los:=los)(nts:=nts); eauto.
+    eapply GenericValue_helper.lift_op1__getTypeSizeInBits with (los:=los)(nts:=nts); eauto.
       intros x y J4 J5.
       unfold mget' in J5.
       unfold getTypeSizeInBits_and_Alignment,
@@ -1521,15 +1452,8 @@ Proof.
         end.
         rewrite J2 in J7. inv J7. auto.
 
-    match goal with
-    | H3: lift_op1 _ _ _ _ = _ |- _ =>
-      inv Hwfg;
-      eapply GVsSig.(lift_op1__inhabited) in H3;
-        try solve [eauto | eapply mget'_is_total; eauto]
-    end.
-
     intros gv0 Hin.
-    eapply GVsSig.(lift_op1__matches_chunks)with (los:=los)(nts:=nts);
+    eapply GenericValue_helper.lift_op1__matches_chunks with (los:=los)(nts:=nts);
       eauto.
       intros. inv Hwfg. apply H3 in H. eapply mget'_matches_chunks; eauto.
 Qed.
@@ -1561,7 +1485,7 @@ Qed.
 
 Lemma preservation_dbCall_case : forall fid l' fa rt la va lb gvs los
   nts s lc Ps lp
-  (Hinhs : forall gv, In gv gvs -> GVsSig.(inhabited) gv)
+  (Hinhs : forall gv, In gv gvs -> GenericValue_helper.inhabited gv)
   (Huniq: uniqFdef (fdef_intro (fheader_intro fa rt fid la va) lb))
   (HwfF: wf_fdef s (module_intro los nts Ps)
     (fdef_intro (fheader_intro fa rt fid la va) lb))
@@ -1614,7 +1538,7 @@ Lemma preservation_cmd_updated_case : forall
   (lc : GVsMap)
   (gl : GVMap)
   (fs : GVMap)
-  (gv3 : GVs)
+  (gv3 : GenericValue)
   (EC : list ExecutionContext)
   (cs : list cmd)
   (tmn : terminator)
@@ -1659,7 +1583,7 @@ Lemma preservation_cmd_updated_case : forall
             CurBB := B;
             CurCmds := cs;
             Terminator := tmn;
-            Locals := updateAddAL GVs lc id0 gv3;
+            Locals := updateAddAL GenericValue lc id0 gv3;
             Allocas := als |};
      ECS := EC;
      Mem := Mem0 |}.
@@ -1884,7 +1808,7 @@ Lemma wf_ExecutionContext__at_beginning_of_function: forall
   (Ps : products) (HwfSystem : wf_system S)
   (HmInS : moduleInSystemB (module_intro los nts Ps) S = true)
   (fid : id) (lp : params) (lc' : GVsMap) (l' : l) (ps' : phinodes)
-  (cs' : cmds) (tmn' : terminator) f (gvs : list GVs)
+  (cs' : cmds) (tmn' : terminator) f (gvs : list GenericValue)
   (H2 : getEntryBlock f = ret (l', stmts_intro ps' cs' tmn'))
   (H4 : initLocals (los, nts) (getArgsOfFdef f) gvs = ret lc')
   (HFinPs' : InProductsB (product_fdef f) Ps = true)
@@ -2017,7 +1941,7 @@ Case "sReturn".
         destruct R1; try solve [inv H1].
         destruct R.
           destruct n; inv HeqR.
-          remember (GVsSig.(lift_op1) (fit_gv (los, nts) rt) g rt) as R2.
+          remember (GenericValue_helper.lift_op1 (fit_gv (los, nts) rt) g rt) as R2.
           destruct R2; inv H1.
           inv Hwfc.
 
@@ -2045,7 +1969,7 @@ Case "sReturn".
         destruct R1; try solve [inv H1].
         destruct R.
           destruct n; inv HeqR.
-          remember (GVsSig.(lift_op1) (fit_gv (los, nts) rt) g rt) as R2.
+          remember (GenericValue_helper.lift_op1 (fit_gv (los, nts) rt) g rt) as R2.
           destruct R2; inv H1.
           inv Hwfc.
           match goal with
@@ -2262,12 +2186,11 @@ Case "sMalloc". eapply preservation_cmd_updated_case in HwfS1; simpl; eauto.
   eapply wf_GVs_intro; eauto.
     unfold getTypeSizeInBits. simpl. eauto.
     intros gv Hin.
-    apply GVsSig.(none_undef2gvs_inv) in Hin; subst; auto.
+    apply GenericValue_helper.none_undef2gvs_inv in Hin; subst; auto.
       intros mc. congruence.
-    apply GVsSig.(gv2gvs__inhabited).
 
     intros gv Hin. unfold gv_chunks_match_typ, vm_matches_typ.
-    apply GVsSig.(none_undef2gvs_inv) in Hin; subst; simpl.
+    apply GenericValue_helper.none_undef2gvs_inv in Hin; subst; simpl.
     constructor; auto. simpl. split; auto.
       intros mc. congruence.
 
@@ -2284,12 +2207,11 @@ Case "sAlloca". eapply preservation_cmd_updated_case in HwfS1; simpl; eauto.
   eapply wf_GVs_intro; eauto.
     unfold getTypeSizeInBits. simpl. eauto.
     intros gv Hin.
-    apply GVsSig.(none_undef2gvs_inv) in Hin; subst; auto.
+    apply GenericValue_helper.none_undef2gvs_inv in Hin; subst; auto.
       intros mc. congruence.
-    apply GVsSig.(gv2gvs__inhabited).
 
     intros gv Hin. unfold gv_chunks_match_typ, vm_matches_typ.
-    apply GVsSig.(none_undef2gvs_inv) in Hin; subst; simpl.
+    apply GenericValue_helper.none_undef2gvs_inv in Hin; subst; simpl.
     constructor; auto. simpl. split; auto.
       intros mc. congruence.
 
@@ -2311,13 +2233,11 @@ Case "sLoad".  eapply preservation_cmd_updated_case in HwfS1; simpl; eauto.
     remember (getTypeSizeInBits_and_Alignment (los, nts) true t) as R.
     destruct R as [[]|]; inv J1.
     unfold getTypeSizeInBits_and_Alignment in HeqR.
-    eapply GVsSig.(gv2gvs__getTypeSizeInBits); eauto.
-
-    apply GVsSig.(gv2gvs__inhabited).
+    eapply GenericValue_helper.gv2gvs__getTypeSizeInBits; eauto.
 
     intros gv0 Hin.
     eapply mload__matches_chunks in H1'; eauto.
-    eapply GVsSig.(gv2gvs__matches_chunks); eauto.
+    eapply GenericValue_helper.gv2gvs__matches_chunks; eauto.
 
 Case "sStore". eapply preservation_cmd_non_updated_case in HwfS1; eauto.
 Case "sGEP".
@@ -2500,7 +2420,7 @@ Qed.
 Lemma const2GV_isnt_stuck : forall TD S gl c t,
   wf_const S TD c t ->
   wf_global TD S gl ->
-  exists gv, @const2GV GVsSig TD gl c = Some gv.
+  exists gv, const2GV TD gl c = Some gv.
 Proof.
   intros.
   destruct const2GV_isnt_stuck_mutind as [J _].
@@ -2537,7 +2457,7 @@ Lemma getOperandValue_inCmdOps_isnt_stuck : forall
   (Hinscope : wf_defs (los,nts) f lc l0)
   (v : value)
   (Hvincs : valueInCmdOperands v c),
-  exists gv : GVs,
+  exists gv : GenericValue,
     getOperandValue (los, nts) v lc gl = ret gv.
 Proof.
   intros.
@@ -2587,7 +2507,7 @@ Lemma getOperandValue_inTmnOperans_isnt_stuck : forall
   (Hinscope : wf_defs (los,nts) f lc l0)
   (v : value)
   (Hvincs : valueInTmnOperands v tmn),
-  exists gv : GVs, getOperandValue (los, nts) v lc gl = ret gv.
+  exists gv : GenericValue, getOperandValue (los, nts) v lc gl = ret gv.
 Proof.
   intros.
   destruct v as [vid | vc].
@@ -2695,7 +2615,7 @@ Lemma wf_phinodes__getIncomingValuesForBlockFromPHINodes : forall
          (l0, stmts_intro ps' cs' tmn') ps2)
   (Hsucc : In l0 (successors_terminator tmn1))
   (Hin: exists ps1, ps' = ps1 ++ ps2),
-   exists RVs : list (id * GVs),
+   exists RVs : list (id * GenericValue),
      getIncomingValuesForBlockFromPHINodes (los, nts) ps2
        (l1, stmts_intro ps1 cs1 tmn1) gl lc =
        ret RVs.
@@ -2827,7 +2747,7 @@ Lemma initializeFrameValues__total_aux : forall los nts s fattr ft fid va
   la2 la1 lc1
   (HwfF: wf_fheader s (los, nts) (fheader_intro fattr ft fid (la1 ++ la2) va))
   gvs2,
-  exists lc2, @_initializeFrameValues GVsSig (los,nts) la2 gvs2 lc1 = Some lc2.
+  exists lc2, _initializeFrameValues (los,nts) la2 gvs2 lc1 = Some lc2.
 Proof.
   induction la2; simpl in *; intros.
     eauto.
@@ -2854,9 +2774,9 @@ Proof.
       apply IHla2 with (gvs2:=gvs2)(lc1:=lc1) in HwfF'.
       destruct HwfF' as [lc2 J'].
       rewrite J'.
-      assert (exists gvs2, GVsSig.(lift_op1) (fit_gv (los, nts) t) g t
+      assert (exists gvs2, GenericValue_helper.lift_op1 (fit_gv (los, nts) t) g t
         = Some gvs2) as W.
-        apply GVsSig.(lift_op1__isnt_stuck); eauto using fit_gv__total.
+        apply GenericValue_helper.lift_op1__isnt_stuck; eauto using fit_gv__total.
       destruct W as [gvs2' W].
       rewrite W. eauto.
 Qed.
@@ -2865,14 +2785,14 @@ Lemma initLocal__total : forall los nts Ps s fattr ft fid va bs2 la2
   (HwfF: wf_fdef s (module_intro los nts Ps)
     (fdef_intro (fheader_intro fattr ft fid la2 va) bs2))
   gvs2,
-  exists lc2, @initLocals GVsSig (los,nts) la2 gvs2 = Some lc2.
+  exists lc2, initLocals (los,nts) la2 gvs2 = Some lc2.
 Proof.
   intros.
   unfold initLocals. inv HwfF.
   eapply initializeFrameValues__total_aux with (la1:=nil); eauto.
 Qed.
 
-Ltac gvs_inhabited_inv H := apply GVsSig.(inhabited_inv) in H; inv H.
+Ltac gvs_inhabited_inv H := apply GenericValue_helper.inhabited_inv in H; inv H.
 
 Lemma wf_params_spec' : forall TD gvss lp,
   wf_params TD gvss lp ->
@@ -3081,7 +3001,7 @@ Proof.
     destruct_tmn tmn.
     SCase "tmn=ret".
       simpl in HwfCall.
-      assert (exists gv : GVs,
+      assert (exists gv : GenericValue,
         getOperandValue (los, nts) value5 lc gl = ret gv) as H.
         eapply getOperandValue_inTmnOperans_isnt_stuck; eauto.
          simpl. auto.
@@ -3120,10 +3040,10 @@ Proof.
             | H6: module_intro _ _ _ = module_intro _ _ _ |- _ => inv H6
             end.
             assert (exists gvs2,
-              GVsSig.(lift_op1) (fit_gv (layouts5, namedts5) rt0) gv rt0
+              GenericValue_helper.lift_op1 (fit_gv (layouts5, namedts5) rt0) gv rt0
                 = Some gvs2) as W.
               match goal with | H19: wf_insn_base _ _ _ |- _ => inv H19 end.
-              apply GVsSig.(lift_op1__isnt_stuck); eauto using fit_gv__total.
+              apply GenericValue_helper.lift_op1__isnt_stuck; eauto using fit_gv__total.
             destruct W as [gvs2' W]. rewrite W.
             eauto.
 
@@ -3169,7 +3089,6 @@ Proof.
       assert (exists c, c @ cond) as Hinh.
         inv Hwfc.
         eapply getOperandValue__inhabited in Hget; eauto.
-        gvs_inhabited_inv Hget. eauto.
       destruct Hinh as [c Hinh].
       assert (exists sts',
               Some sts' =
@@ -3298,7 +3217,7 @@ Proof.
       destruct J0 as [gv0 J0].
       rewrite J. rewrite J0.
       inv Hwfc. apply wf_value__wf_typ in H6. destruct H6.
-      apply GVsSig.(lift_op2__isnt_stuck); eauto using mbop_is_total.
+      apply GenericValue_helper.lift_op2__isnt_stuck; eauto using mbop_is_total.
       eauto.
     destruct Hinsn_bop as [gv3 Hinsn_bop].
     exists
@@ -3332,7 +3251,7 @@ Proof.
       destruct J0 as [gv0 J0].
       rewrite J. rewrite J0.
       inv Hwfc. apply wf_value__wf_typ in H6. destruct H6.
-      apply GVsSig.(lift_op2__isnt_stuck); eauto using mfbop_is_total.
+      apply GenericValue_helper.lift_op2__isnt_stuck; eauto using mfbop_is_total.
       eauto.
 
     destruct Hinsn_fbop as [gv3 Hinsn_fbop].
@@ -3365,7 +3284,7 @@ Proof.
       | H12: exists _:_, _ |- _ => destruct H12 as [idxs [o [J1 J2]]]
       end.
       rewrite J1. rewrite J2.
-      apply GVsSig.(lift_op1__isnt_stuck); eauto using mget'_is_total.
+      apply GenericValue_helper.lift_op1__isnt_stuck; eauto using mget'_is_total.
       eauto.
     destruct J' as [gv' J'].
     exists
@@ -3406,7 +3325,7 @@ Proof.
       | H9: wf_value _ _ _ _ ?t0 |- context [mset' _ _ ?t0 _] =>
         apply wf_value__wf_typ in H9; destruct H9
       end.
-      apply GVsSig.(lift_op2__isnt_stuck); eauto using mset'_is_total.
+      apply GenericValue_helper.lift_op2__isnt_stuck; eauto using mset'_is_total.
     destruct J'' as [gv'' J''].
     exists
          {|
@@ -3437,7 +3356,6 @@ Proof.
     destruct J as [gvs J].
     assert (exists gn, gn @ gvs) as Hinh.
       eapply getOperandValue__inhabited in J; eauto.
-      gvs_inhabited_inv J. eauto.
     destruct Hinh as [gn Hinh].
     remember (malloc (los, nts) M asz gn a) as R.
     destruct R as [[M' mb] |].
@@ -3472,7 +3390,6 @@ Proof.
     assert (exists gv, gv @ gvs) as Hinh.
       inv Hwfc.
       eapply getOperandValue__inhabited in J; eauto.
-      gvs_inhabited_inv J. eauto.
     destruct Hinh as [gv Hinh].
     remember (free (los, nts) M gv) as R.
     destruct R as [M'|].
@@ -3511,7 +3428,6 @@ Proof.
     destruct J as [gvs J].
     assert (exists gn, gn @ gvs) as Hinh.
       eapply getOperandValue__inhabited in J; eauto.
-      gvs_inhabited_inv J. eauto.
     destruct Hinh as [gn Hinh].
     remember (malloc (los, nts) M asz gn a) as R.
     destruct R as [[M' mb] |].
@@ -3547,7 +3463,6 @@ Proof.
     assert (exists gv, gv @ gvs) as Hinh.
       inv Hwfc.
       eapply getOperandValue__inhabited in J; eauto.
-      gvs_inhabited_inv J. eauto.
     destruct Hinh as [gv Hinh].
     remember (mload (los,nts) M gv t a) as R.
     destruct R as [gv' |].
@@ -3586,11 +3501,9 @@ Proof.
     inv Hwfc.
     assert (exists gv, gv @ gvs) as Hinh1.
       eapply getOperandValue__inhabited in J; eauto.
-      gvs_inhabited_inv J. eauto.
     destruct Hinh1 as [gv Hinh1].
     assert (exists mgv, mgv @ mgvs) as Hinh2.
       eapply getOperandValue__inhabited in J0; eauto.
-      gvs_inhabited_inv J0. eauto.
     destruct Hinh2 as [mgv Hinh2].
     remember (mstore (los,nts) M mgv t gv a) as R.
     destruct R as [M' |].
@@ -3634,7 +3547,7 @@ Proof.
       destruct Hins as [vidxs Hins]
     end.
     assert (exists mp', GEP (los, nts) t mp vidxs i1 typ' = Some mp') as J3.      unfold GEP, gep.
-      apply GVsSig.(lift_op1__isnt_stuck); eauto using GEP_is_total.
+      apply GenericValue_helper.lift_op1__isnt_stuck; eauto using GEP_is_total.
     destruct J3 as [mp' J3].
     left.
     exists
@@ -3662,7 +3575,7 @@ Proof.
           simpl; auto.
       destruct J as [gv J].
       rewrite J. inv Hwfc.
-      apply GVsSig.(lift_op1__isnt_stuck); eauto using mtrunc_is_total.
+      apply GenericValue_helper.lift_op1__isnt_stuck; eauto using mtrunc_is_total.
 
     destruct Hinsn_trunc as [gv2 Hinsn_trunc].
     exists
@@ -3690,7 +3603,7 @@ Proof.
           simpl; auto.
       destruct J as [gv J].
       rewrite J. inv Hwfc.
-      apply GVsSig.(lift_op1__isnt_stuck); eauto using mext_is_total.
+      apply GenericValue_helper.lift_op1__isnt_stuck; eauto using mext_is_total.
 
     destruct Hinsn_ext as [gv2 Hinsn_ext].
     exists
@@ -3718,7 +3631,7 @@ Proof.
           simpl; auto.
       destruct J as [gv J].
       rewrite J. inv Hwfc.
-      apply GVsSig.(lift_op1__isnt_stuck); eauto using mcast_is_total.
+      apply GenericValue_helper.lift_op1__isnt_stuck; eauto using mcast_is_total.
 
     destruct Hinsn_cast as [gv2 Hinsn_cast].
     exists
@@ -3756,7 +3669,7 @@ Proof.
       | H11: wf_value _ _ _ _ _ |- _ =>
         apply wf_value__wf_typ in H11; destruct H11
       end.
-      apply GVsSig.(lift_op2__isnt_stuck); eauto using micmp_is_total.
+      apply GenericValue_helper.lift_op2__isnt_stuck; eauto using micmp_is_total.
 
     destruct Hinsn_icmp as [gv2 Hinsn_icmp].
     exists
@@ -3794,7 +3707,7 @@ Proof.
       | H11: wf_value _ _ _ _ _ |- _ =>
         apply wf_value__wf_typ in H11; destruct H11
       end.
-      apply GVsSig.(lift_op2__isnt_stuck); eauto using mfcmp_is_total.
+      apply GenericValue_helper.lift_op2__isnt_stuck; eauto using mfcmp_is_total.
 
     destruct Hinsn_fcmp as [gv2 Hinsn_fcmp].
     exists
@@ -3820,7 +3733,6 @@ Proof.
     assert (exists c, c @ cond) as Hinh.
       inv Hwfc.
       eapply getOperandValue__inhabited in J; eauto.
-      gvs_inhabited_inv J. eauto.
     destruct Hinh as [c Hinh].
     assert (exists gv0, getOperandValue (los, nts) v0 lc gl = Some gv0)
       as J0.
@@ -3862,7 +3774,6 @@ Proof.
     assert (exists fptr, fptr @ fptrs) as Hinh.
       inv Hwfc.
       eapply getOperandValue__inhabited in J'; eauto.
-      gvs_inhabited_inv J'. eauto.
     destruct Hinh as [fptr Hinh].
     remember (lookupFdefViaPtr ps fs fptr) as Hlk.
     destruct Hlk as [f' |].
