src/Vellvm/vellvm.v
@@ -20,7 +20,6 @@ Require Export static.
 Require Export opsem.
 Require Export opsem_wf.
 Require Export dopsem.
-Require Export ndopsem.
 Require Export external_intrinsics.
 Require Export vellvm_tactics.
 
